Make everything precompilable
Disables `extract_closed` where initialization is required

src/lean/Pod/Fixnum.lean
@@ -1,1 +1,173 @@
-import PodPrecompiled.Fixnum
+import Pod.Meta
+import Pod.Storable
+import Pod.UInt
+
+namespace Pod
+
+def UFixnum.bitWidth := (System.Platform.numBits - 1)
+
+abbrev UFixnum.size : Nat := (2 ^ UFixnum.bitWidth) - 1 + 1
+
+theorem UFixnum.size_eq : Or (UFixnum.size = 2147483648) (UFixnum.size = 9223372036854775808) :=
+  show Or ((Nat.succ (Nat.sub (2 ^ (System.Platform.numBits - 1)) 1)) = 2147483648) (Eq (Nat.succ (Nat.sub (2 ^ (System.Platform.numBits - 1)) 1)) 9223372036854775808) from
+  match System.Platform.numBits, System.Platform.numBits_eq with
+  | _, Or.inl rfl => Or.inl (by decide)
+  | _, Or.inr rfl => Or.inr (by decide)
+
+theorem UFixnum.size_ge : UFixnum.size ≥ 2147483648 :=
+  match UFixnum.size_eq with
+  | .inl h => Nat.le_of_eq h.symm
+  | .inr h => Nat.le_trans (by decide) (Nat.le_of_eq h.symm)
+
+theorem UFixnum.bitWidth_ge : UFixnum.bitWidth ≥ 31 := by
+  unfold bitWidth
+  cases System.Platform.numBits_eq
+  case inl h => rewrite [h]; decide
+  case inr h => rewrite [h]; decide
+
+/--
+A `UFixnum` is the largest unsigned integer type stored unboxed.
+
+For example, if running on a 32-bit machine, UFixnum is equivalent to UInt31.
+Or on a 64-bit machine, UInt63.
+-/
+structure UFixnum where
+  val : Fin UFixnum.size
+deriving Repr, Inhabited, DecidableEq
+
+def UFixnum.maximum : UFixnum :=
+  ⟨(2 ^ bitWidth - 1), Nat.lt_succ_self _⟩
+
+def UFixnum.ofNatCore (x : Nat) (h : x < size) : UFixnum :=
+  ⟨x, h⟩
+
+def UFixnum.ofNatCore' (x : Nat) (h : x < 2147483648) : UFixnum :=
+  ⟨x, Nat.lt_of_lt_of_le h size_ge⟩
+
+private unsafe
+def UFixnum.ofNatImpl (x : Nat) : UFixnum :=
+  ⟨(x &&& ((1 <<< (System.Platform.numBits - 1)) - 1)), lcProof⟩
+
+@[implemented_by ofNatImpl]
+def UFixnum.ofNat (x : Nat) : UFixnum :=
+  .mk $ Fin.ofNat' x (Nat.lt_of_lt_of_le (by decide) size_ge)
+
+instance UFixnum.instOfNat {n} : OfNat UFixnum n := ⟨.ofNat n⟩
+
+@[extern c inline "lean_box(#1)"]
+def UFixnum.ofBool (x : Bool) : UFixnum :=
+  cond x 1 0
+
+def UFixnum.ofUInt8 (x : UInt8) : UFixnum :=
+  ⟨x.toNat, Nat.lt_trans x.val.isLt $ Nat.lt_of_lt_of_le (by decide) size_ge⟩
+
+def UFixnum.ofUInt16 (x : UInt16) : UFixnum :=
+  ⟨x.toNat, Nat.lt_trans x.val.isLt $ Nat.lt_of_lt_of_le (by decide) size_ge⟩
+
+@[extern c inline "lean_box(#1 & (((size_t)1 << ((sizeof(size_t) * 8) - 1)) - 1))"]
+opaque UFixnum.ofUInt32 (x : UInt32) : UFixnum
+
+@[extern c inline "lean_box(#1 & (((size_t)1 << ((sizeof(size_t) * 8) - 1)) - 1))"]
+opaque UFixnum.ofUInt64 (x : UInt64) : UFixnum
+
+@[inline]
+def UFixnum.toNat (x : UFixnum) : Nat :=
+  x.val.val
+
+theorem UFixnum.toNat_lt (x : UFixnum) : x.toNat < 9223372036854775808 :=
+  match UFixnum.size_eq with
+  | .inl h => Nat.lt_trans x.val.isLt (by rewrite [h]; decide)
+  | .inr h => h ▸ x.val.isLt
+
+@[extern c inline "((size_t)#1 >> 1) != 0"]
+def UFixnum.toBool (x : UFixnum) : Bool :=
+  x.toNat != 0
+
+@[extern c inline "lean_unbox(#1)"]
+opaque UFixnum.toUInt8 (x : UFixnum) : UInt8
+
+@[extern c inline "lean_unbox(#1)"]
+opaque UFixnum.toUInt16 (x : UFixnum) : UInt16
+
+@[extern c inline "lean_unbox(#1)"]
+def UFixnum.toUInt32 (x : UFixnum) : UInt32 :=
+  x.toNat.toUInt32
+
+@[extern c inline "lean_unbox(#1)"]
+def UFixnum.toUInt64 (x : UFixnum) : UInt64 :=
+  UInt64.ofNatCore x.toNat (Nat.lt_trans (toNat_lt x) (by decide))
+
+@[extern c inline "#1 == #2"]
+def UFixnum.beq (x y : UFixnum) : Bool :=
+  x.toNat == y.toNat
+
+@[extern c inline "(size_t)#1 < (size_t)#2"]
+def UFixnum.blt (x y : UFixnum) : Bool :=
+  x.toNat < y.toNat
+
+@[extern c inline "(size_t)#1 <= (size_t)#2"]
+def UFixnum.ble (x y : UFixnum) : Bool :=
+  x.toNat <= y.toNat
+
+@[extern c inline "(void*)(((size_t)#1 ^ (size_t)#2) | 1)"]
+def UFixnum.xor (x y : UFixnum) : UFixnum :=
+  .mk <| x.val.xor y.val
+
+@[extern c inline "(void*)((size_t)#1 | (size_t)#2)"]
+def UFixnum.lor (x y : UFixnum) : UFixnum :=
+  .mk <| x.val.lor y.val
+
+@[extern c inline "(void*)((size_t)#1 & (size_t)#2)"]
+def UFixnum.land (x y : UFixnum) : UFixnum :=
+  .mk <| x.val.land y.val
+
+@[extern c inline "(void*)(~(size_t)#1)"]
+opaque UFixnum.complement (x : UFixnum) : UFixnum
+
+@[extern c inline "lean_box(lean_unbox(#1) << (lean_unbox(#2) % (sizeof(size_t) * 8)))"]
+opaque UFixnum.shiftLeft (x y : UFixnum) : UFixnum
+
+@[extern c inline "lean_box(lean_unbox(#1) >> (lean_unbox(#2) % (sizeof(size_t) * 8)))"]
+opaque UFixnum.shiftRight (x y : UFixnum) : UFixnum
+
+@[extern c inline "lean_box(lean_unbox(#1) + lean_unbox(#2))"]
+def UFixnum.add (x y : UFixnum) : UFixnum :=
+  .mk <| x.val + y.val
+
+@[extern c inline "lean_box(lean_unbox(#1) - lean_unbox(#2))"]
+def UFixnum.sub (x y : UFixnum) : UFixnum :=
+  .mk <| x.val - y.val
+
+@[extern c inline "lean_box(lean_unbox(#1) * lean_unbox(#2))"]
+def UFixnum.mul (x y : UFixnum) : UFixnum :=
+  .mk <| x.val * y.val
+
+@[extern c inline "(lean_unbox(#2) == 0) ? lean_box(0) : (lean_box(lean_unbox(#1) / lean_unbox(#2)))"]
+def UFixnum.div (x y : UFixnum) : UFixnum :=
+  .mk <| x.val / y.val
+
+@[extern c inline "(lean_unbox(#2) == 0) ? #1 : (lean_box(lean_unbox(#1) % lean_unbox(#2)))"]
+def UFixnum.mod (x y : UFixnum) : UFixnum :=
+  .mk <| x.val % y.val
+
+instance : BEq UFixnum := ⟨UFixnum.beq⟩
+instance : Xor UFixnum := ⟨UFixnum.xor⟩
+instance : OrOp UFixnum := ⟨UFixnum.lor⟩
+instance : AndOp UFixnum := ⟨UFixnum.land⟩
+instance : Complement UFixnum := ⟨UFixnum.complement⟩
+instance : ShiftLeft UFixnum := ⟨UFixnum.shiftLeft⟩
+instance : ShiftRight UFixnum := ⟨UFixnum.shiftRight⟩
+instance : Add UFixnum := ⟨UFixnum.add⟩
+instance : Sub UFixnum := ⟨UFixnum.sub⟩
+instance : Mul UFixnum := ⟨UFixnum.mul⟩
+instance : Div UFixnum := ⟨UFixnum.div⟩
+instance : Mod UFixnum := ⟨UFixnum.mod⟩
+
+instance : ToString UFixnum where
+  toString x := toString x.toNat
+
+instance : Storable UFixnum where
+  byteSize := byteSize USize
+  alignment := alignment USize
+  alignment_dvd_byteSize := alignment_dvd_byteSize
+  byteSize_gt_zero := byteSize_gt_zero
