src/lean/Pod.lean
@@ -1,4 +1,11 @@
-import PodPrecompiled
+import Pod.Meta
+import Pod.Lemmas
+import Pod.Endianness
+import Pod.Storable
+import Pod.UInt
+import Pod.Fixnum
+import Pod.Int
+import Pod.Float
 import Pod.Initialization
 import Pod.OnFinalize
 import Pod.BytesView
