src/lean/Pod/UInt.lean
@@ -1,1 +1,89 @@
-import PodPrecompiled.UInt
+import Pod.Endianness
+
+@[extern c inline "#1"]
+def UInt8.ofBool (x : Bool) : UInt8 := cond x 1 0
+
+@[extern "lean_pod_UInt16_bswap"]
+def UInt16.bswap (value : UInt16) : UInt16 :=
+  (value <<< 8) ||| (value >>> 8)
+
+@[extern "lean_pod_UInt16_toBigEndian"]
+def UInt16.toBigEndian (value : UInt16) :=
+  if Pod.endianness = .big
+    then value
+    else value.bswap
+
+@[extern "lean_pod_UInt16_toLittleEndian"]
+def UInt16.toLittleEndian (value : UInt16) :=
+  if Pod.endianness = .little
+    then value
+    else value.bswap
+
+@[extern c inline "(uint16_t)#1"]
+def UInt16.ofBool (x : Bool) : UInt16 := cond x 1 0
+
+@[extern "lean_pod_UInt32_bswap"]
+def UInt32.bswap (value : UInt32) : UInt32 :=
+  ((value &&& 0x000000FF) <<< 24) |||
+  ((value &&& 0x0000FF00) <<<  8) |||
+  ((value &&& 0x00FF0000) >>>  8) |||
+  ((value &&& 0xFF000000) >>> 24)
+
+@[extern "lean_pod_UInt32_toBigEndian"]
+def UInt32.toBigEndian (value : UInt32) :=
+  if Pod.endianness = .big
+    then value
+    else value.bswap
+
+@[extern "lean_pod_UInt32_toLittleEndian"]
+def UInt32.toLittleEndian (value : UInt32) :=
+  if Pod.endianness = .little
+    then value
+    else value.bswap
+
+@[extern c inline "(uint32_t)#1"]
+def UInt32.ofBool (x : Bool) : UInt32 := cond x 1 0
+
+@[extern "lean_pod_UInt64_bswap"]
+def UInt64.bswap (value : UInt64) : UInt64 :=
+  ((value &&& 0xFF00000000000000) >>> 56) |||
+  ((value &&& 0x00FF000000000000) >>> 40) |||
+  ((value &&& 0x0000FF0000000000) >>> 24) |||
+  ((value &&& 0x000000FF00000000) >>>  8) |||
+  ((value &&& 0x00000000FF000000) <<<  8) |||
+  ((value &&& 0x0000000000FF0000) <<< 24) |||
+  ((value &&& 0x000000000000FF00) <<< 40) |||
+  ((value &&& 0x00000000000000FF) <<< 56)
+
+@[extern "lean_pod_UInt64_toBigEndian"]
+def UInt64.toBigEndian (value : UInt64) :=
+  if Pod.endianness = .big
+    then value
+    else value.bswap
+
+@[extern "lean_pod_UInt64_toLittleEndian"]
+def UInt64.toLittleEndian (value : UInt64) :=
+  if Pod.endianness = .little
+    then value
+    else value.bswap
+
+@[extern c inline "(uint64_t)#1"]
+def UInt64.ofBool (x : Bool) : UInt64 := cond x 1 0
+
+@[extern "lean_pod_USize_bswap"]
+opaque USize.bswap (value : USize) : USize
+
+@[extern "lean_pod_USize_toBigEndian"]
+def USize.toBigEndian (value : USize) :=
+  if Pod.endianness = .big
+    then value
+    else value.bswap
+
+@[extern "lean_pod_USize_toLittleEndian"]
+def USize.toLittleEndian (value : USize) :=
+  if Pod.endianness = .little
+    then value
+    else value.bswap
+
+@[extern c inline "(size_t)#1"]
+def USize.ofBool (x : Bool) : USize := cond x (USize.ofNat32 1 $ by decide) (USize.ofNat32 0 $ by decide)
