src/lean/PodPrecompiled.lean
@@ -1,8 +1,0 @@
-import PodPrecompiled.Meta
-import PodPrecompiled.Lemmas
-import PodPrecompiled.Endianness
-import PodPrecompiled.Storable
-import PodPrecompiled.UInt
-import PodPrecompiled.Fixnum
-import PodPrecompiled.Int
-import PodPrecompiled.Float
